sondeos/core_after.lean
@@ -1,0 +1,9 @@
+import PeanoRF.HA.Numerals
+import PeanoRF.HA.Arith
+#print axioms PeanoRF.HA.ctx
+#print axioms PeanoRF.HA.zero_add
+#print axioms PeanoRF.HA.succ_add
+#print axioms PeanoRF.HA.induction_object
+#print axioms PeanoRF.HA.numeralI_add
+#print axioms PeanoRF.HA.numeralI_pow
+#print axioms PeanoRF.HA.closed_term_eq_numeral
